simplify
git-svn-id: https://projects.brucker.ch/hol-testgen/svn/HOL-TestGen/trunk/hol-testgen@10950 3260e6d1-4efc-4170-b0a7-36055960796d

src/compiler/meta/OCL_compiler_meta_META.thy
@@ -56,26 +56,22 @@ datatype ocl_flush_all = OclFlushAll
 
 (* *)
 
-type_synonym ocl2_class_raw = ocl_class_raw
-type_synonym ocl2_ass_class = ocl_ass_class
-type_synonym ocl2_ctxt_pre_post = ocl_ctxt_pre_post
-type_synonym ocl2_ctxt_inv = ocl_ctxt_inv
+datatype floor = Floor1 | Floor2 | Floor3
 
 (* *)
 
 (* le meta-model de "tout le monde" - frederic. *)
-datatype ocl_deep_embed_ast = (* USE *)
-                              OclAstClassRaw ocl_class_raw
-                            | OclAstAssociation ocl_association
-                            | OclAstAssClass ocl_ass_class
-                            | OclAstCtxtPrePost ocl_ctxt_pre_post
-                            | OclAstCtxtInv ocl_ctxt_inv
+datatype ocl_deep_embed_ast =
+  (* For the following constructors, if they are preceded by an additional
+     'floor' field, then it indicates the degre of reflection
+     (otherwise degre = 1 by default). *)
 
-                              (* USE reflected 1 time *)
-                            | Ocl2AstClassRaw ocl2_class_raw
-                            | Ocl2AstAssClass ocl2_ass_class
-                            | Ocl2AstCtxtPrePost ocl2_ctxt_pre_post
-                            | Ocl2AstCtxtInv ocl2_ctxt_inv
+                              (* USE *)
+                              OclAstClassRaw floor ocl_class_raw
+                            | OclAstAssociation ocl_association
+                            | OclAstAssClass floor ocl_ass_class
+                            | OclAstCtxtPrePost floor ocl_ctxt_pre_post
+                            | OclAstCtxtInv floor ocl_ctxt_inv
 
                               (* invented *)
                             | OclAstInstance ocl_instance
@@ -118,8 +114,8 @@ record ocl_compiler_config =  D_disable_thy_output :: bool
 subsection{* Auxilliary *}
 
 definition "map2_ctxt_term f = (\<lambda>
-    Ocl2AstCtxtPrePost ocl \<Rightarrow> Ocl2AstCtxtPrePost (Ctxt_expr_update (List_map (\<lambda>(s, x). (s, f x))) ocl)
-  | Ocl2AstCtxtInv ocl \<Rightarrow> Ocl2AstCtxtInv (Ctxt_inv_expr_update (List_map (\<lambda>(s, x). (s, f x))) ocl)
+    OclAstCtxtPrePost Floor2 ocl \<Rightarrow> OclAstCtxtPrePost Floor2 (Ctxt_expr_update (List_map (\<lambda>(s, x). (s, f x))) ocl)
+  | OclAstCtxtInv Floor2 ocl \<Rightarrow> OclAstCtxtInv Floor2 (Ctxt_inv_expr_update (List_map (\<lambda>(s, x). (s, f x))) ocl)
   | x \<Rightarrow> x)"
 
 definition "ocl_compiler_config_more_map f ocl =
